@prefix rdf: <http://www.w3.org/1999/02/22-rdf-syntax-ns#> .
@prefix rdfs: <http://www.w3.org/2000/01/rdf-schema#> .
@prefix schema: <https://schema.org/> .
@prefix croissant: <http://mlcommons.org/croissant/> .
@prefix rai: <http://mlcommons.org/croissant/RAI/> .

# Dataset level properties

rai:dataCollection a rdf:Property ;
  rdfs:label "dataCollection" ;
  rdfs:comment "Description of the data collection process." ;
  schema:domainIncludes schema:Dataset ;
  schema:rangeIncludes schema:Text .

rai:dataCollectionType a rdf:Property ;
  rdfs:label "dataCollectionType" ;
  rdfs:comment "Define the data collection type. Recommended values: Surveys, Secondary Data analysis, Physical data collection, Direct measurement, Document analysis, Manual Human Curator, Software Collection, Experiments, Web Scraping, Web API, Focus groups, Self-reporting, Customer feedback data, User-generated content data, Passive Data Collection, Others." ;
  schema:domainIncludes schema:Dataset ;
  schema:rangeIncludes schema:Text .

rai:dataCollectionMissingData a rdf:Property ;
  rdfs:label "dataCollectionMissingData" ;
  rdfs:comment "Description of missing data in structured/unstructured form." ;
  schema:domainIncludes schema:Dataset ;
  schema:rangeIncludes schema:Text .

rai:dataCollectionRawData a rdf:Property ;
  rdfs:label "dataCollectionRawData" ;
  rdfs:comment "Description of the raw data i.e. source of the data." ;
  schema:domainIncludes schema:Dataset ;
  schema:rangeIncludes schema:Text .

rai:dataCollectionTimeframe a rdf:Property ;
  rdfs:label "dataCollectionTimeframe" ;
  rdfs:comment "Timeframe in terms of start and end date of the collection process, that it described as a DateTime indicating a time period in <a href=\"https://en.wikipedia.org/wiki/ISO_8601#Time_intervals\">ISO 8601 time interval format</a>. For example, a collection time frame ranging from 2020 - 2022 can be indicated in ISO 8601 interval format via \"2020/2022\"." ;
  schema:domainIncludes schema:Dataset ;
  schema:rangeIncludes schema:DateTime .

rai:dataPreprocessingProtocol a rdf:Property ;
  rdfs:label "dataPreprocessingProtocol" ;
  rdfs:comment "Description of the steps that were required to bring collected data to a state that can be processed by an ML model/algorithm, e.g. filtering out incomplete entries etc, if applicable." ;
  schema:domainIncludes schema:Dataset ;
  schema:rangeIncludes schema:Text .

rai:dataImputationProtocol a rdf:Property ;
  rdfs:label "dataImputationProtocol" ;
  rdfs:comment "Description of data imputation process, if applicable." ;
  schema:domainIncludes schema:Dataset ;
  schema:rangeIncludes schema:Text .

rai:dataManipulationProtocol a rdf:Property ;
  rdfs:label "dataManipulationProtocol" ;
  rdfs:comment "Description of data manipulation process, if applicable." ;
  schema:domainIncludes schema:Dataset ;
  schema:rangeIncludes schema:Text .

rai:dataReleaseMaintenancePlan a rdf:Property ;
  rdfs:label "dataReleaseMaintenancePlan" ;
  rdfs:comment "Versioning information in terms of the updating timeframe, the maintainers, and the deprecation policies." ;
  schema:domainIncludes schema:Dataset ;
  schema:rangeIncludes schema:Text .

rai:personalSensitiveInformation a rdf:Property ;
  rdfs:label "personalSensitiveInformation" ;
  rdfs:comment "Sensitive Human Attribute(s)- Gender, Socio-economic status, Geography, Language, Age, Culture, Experience or Seniority, Others (please specify), if applicable." ;
  schema:domainIncludes schema:Dataset ;
  schema:rangeIncludes schema:Text .

rai:dataAnnotationProtocol a rdf:Property ;
  rdfs:label "dataAnnotationProtocol" ;
  rdfs:comment "Description of annotations (labels, ratings) produced, including how these were created or authored -  Annotation Workforce Type, Annotation Characteristic(s), Annotation Description(s), Annotation Task(s), Annotation Distribution(s)." ;
  schema:domainIncludes schema:Dataset ;
  schema:rangeIncludes schema:Text .

rai:dataAnnotationPlatform a rdf:Property ;
  rdfs:label "dataAnnotationPlatform" ;
  rdfs:comment "Platform, tool, or library used to collect annotations by human annotators, if applicable." ;
  schema:domainIncludes schema:Dataset ;
  schema:rangeIncludes schema:Text .

rai:dataAnnotationAnalysis a rdf:Property ;
  rdfs:label "dataAnnotationAnalysis" ;
  rdfs:comment "Considerations related to the process of converting the \"raw\" annotations into the labels that are ultimately packaged in a dataset - Uncertainty or disagreement between annotations on each instance as a signal in the dataset, analysis of systematic disagreements between annotators of different socio demographic group,  how the final dataset annotations will relate to individual annotator responses." ;
  schema:domainIncludes schema:Dataset ;
  schema:rangeIncludes schema:Text .

rai:annotationsPerItem a rdf:Property ;
  rdfs:label "annotationsPerItem" ;
  rdfs:comment "Number of human labels per dataset item, if applicable." ;
  schema:domainIncludes schema:Dataset ;
  schema:rangeIncludes schema:Text .

rai:annotatorDemographics a rdf:Property ;
  rdfs:label "annotatorDemographics" ;
  rdfs:comment "List of demographics specifications about the annotators, if applicable." ;
  schema:domainIncludes schema:Dataset ;
  schema:rangeIncludes schema:Text .

rai:machineAnnotationTools a rdf:Property ;
  rdfs:label "machineAnnotationTools" ;
  rdfs:comment "List of software used for data annotation (e.g., concept extraction, NER, and additional characteristics of the tools used for annotation to allow for replication or extension)." ;
  schema:domainIncludes schema:Dataset ;
  schema:rangeIncludes schema:Text .

rai:dataSocialImpact a rdf:Property ;
  rdfs:label "dataSocialImpact" ;
  rdfs:comment "Discussion of social impact, if applicable." ;
  schema:domainIncludes schema:Dataset ;
  schema:rangeIncludes schema:Text .

rai:dataBiases a rdf:Property ;
  rdfs:label "dataBiases" ;
  rdfs:comment "Description of biases in dataset, if applicable." ;
  schema:domainIncludes schema:Dataset ;
  schema:rangeIncludes schema:Text .

rai:dataLimitations a rdf:Property ;
  rdfs:label "dataLimitations" ;
  rdfs:comment "Known limitations - Data generalization limits (e.g related to data distribution, data quality issues, or data sources) and on-recommended uses, if applicable." ;
  schema:domainIncludes schema:Dataset ;
  schema:rangeIncludes schema:Text .

rai:dataUseCases a rdf:Property ;
  rdfs:label "dataUseCases" ;
  rdfs:comment "Dataset Use(s) - Training, Testing, Validation, Development or Production Use, Fine Tuning, Others (please specify), Usage Guidelines. Recommended uses." ;
  schema:domainIncludes schema:Dataset ;
  schema:rangeIncludes schema:Text .
